iris/ProofSysOpenTails.v
@@ -2082,7 +2082,10 @@ Section ProofSysOpenTails.
               with "Hcg Hown Htext Hpc Hitinv Hesck Hslkk Hslkd
                     Hpid Hprocs Hdep Hidev Hiinum Hivalid Hload Hshot Hfrz").
     iIntros (CID3 Hq3 miu) "%Hcsiu Hcg Hown Hpc Hpid Hshr".
-    iDestruct (inode_shr_gen_forget with "Hshr") as "Hshr".
+    iApply fupd_wp.
+    iMod (inode_shr_gen_pin0 ⊤ kk s dev inum gy ltac:(solve_ndisj) Hkk
+            with "Hitinv Hshr") as "Hshr".
+    iModIntro.
     assert (Hpc2 : ret_pc (M2 !!! Regidx Rra : mword 64)
                    = mword_of_int (SO + 0xbe)) by (rewrite HM2ra; pcw).
     iEval (rewrite Hpc2) in "Hpc".
